%%%%%%%%%%%%%%%%%% ARGUMENT LIST %%%%%%%%%%%%%%%%%%%%

\noindent \textbf{Conjunction / Disjunction}

\begin{enumerate}
\setcounter{enumi}{\value{enumi_saved}}
\item $ B\nvdash  A \vee  \neg A $\hfill\emph{ (LEM)}  
\item $ C\vdash  (A \vee  B) \vee  \neg (A \vee  B) $\hfill\emph{ (LEM - Restricted)}  
\item $ A \wedge  \neg A\vdash  B $\hfill\emph{ (LNC)}  
\item $ B\vdash  \neg (A \wedge  \neg A) $\hfill\emph{ (LNC*)}  
\item $ \neg (A \vee  \neg A)\nvdash  A \wedge  \neg A $\hfill\emph{ }  
\item $ B\nvdash  (A \wedge  A) \vee  (\neg A \wedge  \neg A) $\hfill\emph{ }  
\item $ B\nvdash  (A \vee  A) \vee  (\neg A \vee  \neg A) $\hfill\emph{ }  
\item $ A \wedge  B\leftvdash\rightvdash  B \wedge  A $ \hfill\emph{ (Commutation - Conjunction)}  
\item $ A \vee  B\leftvdash\rightvdash  B \vee  A $ \hfill\emph{ (Commutation - Disjunction)}  
\item $ A \wedge  (B \wedge  C)\leftvdash\rightvdash  (A \wedge  B) \wedge  C $ \hfill\emph{ (Association - Conjunction)}  
\item $ A \vee  (B \vee  C)\leftvdash\rightvdash  (A \vee  B) \vee  C $ \hfill\emph{ (Association - Disjunction)}  
\item $ A\leftvdash\rightvdash  A \wedge  A $ \hfill\emph{ (Idempotence - Conjunction)}  
\item $ A\leftvdash\rightvdash  A \vee  A $ \hfill\emph{ (Idempotence - Disjunction)}  
\item $ A \wedge  (B \vee  C)\leftvdash\rightvdash  (A \wedge  B) \vee  (A \wedge  C) $ \hfill\emph{ (Distribution$_1$)}  
\item $ A \vee  (B \wedge  C)\leftvdash\rightvdash  (A \vee  B) \wedge  (A \vee  C) $ \hfill\emph{ (Distribution$_2$)}  
\item $ \{A \vee  B, \neg A \} \vdash  B $\hfill\emph{ (Disjunctive Syllogism)}  
\setcounter{enumi_saved}{\value{enumi}}
\end{enumerate}


%%%%%%%%%%%%%%%%%%%%% TABLEAUX %%%%%%%%%%%%%%%%%%%%%




\begin{quote} 
(1) $ B\nvdash  A \vee  \neg A $
\end{quote} 
\bigskip

\Tree[.{$B, 0\varoplus $ \\ \framebox{$A \vee  \neg A, 0\varominus $} \\ $0\mathcal{R} 0$ \\ \framebox{$\neg (A \vee  \neg A), 0\varoplus $} \\ $A, 0\varominus $ \\ $\neg A, 0\varominus $}  ]

\bigskip

Counter Model: 

\bigskip
\noindent $\mathcal{W} = \{ w_0\} $\\
$\mathcal{R} = \{ \langle w_0,w_0 \rangle \} $\\
$ \mathcal{\nu}_{w_0}(B)=1 $ \\
$ \mathcal{\nu}_{w_0}(A)=.5 $ \\
\bigskip




\begin{quote} 
(2) $ C\vdash  (A \vee  B) \vee  \neg (A \vee  B) $
\end{quote} 
\bigskip

\Tree[.{$C, 0\varoplus $ \\ \framebox{$(A \vee  B) \vee  \neg (A \vee  B), 0\varominus $} \\ $0\mathcal{R} 0$ \\ \framebox{$\neg ((A \vee  B) \vee  \neg (A \vee  B)), 0\varoplus $} \\ \framebox{$A \vee  B, 0\varominus $} \\ $\neg (A \vee  B), 0\varominus $ \\ $\neg (A \vee  B), 0\varoplus $ \\ $ \varotimes  $}  ]


\begin{quote} 
(3) $ A \wedge  \neg A\vdash  B $
\end{quote} 
\bigskip

\Tree[.{\framebox{$A \wedge  \neg A, 0\varoplus $} \\ $B, 0\varominus $ \\ $0\mathcal{R} 0$ \\ $A, 0\varoplus $ \\ $\neg A, 0\varoplus $ \\ $ \varotimes  $}  ]


\begin{quote} 
(4) $ B\vdash  \neg (A \wedge  \neg A) $
\end{quote} 
\bigskip

\Tree[.{$B, 0\varoplus $ \\ \framebox{$\neg (A \wedge  \neg A), 0\varominus $} \\ $0\mathcal{R} 0$ \\ \framebox{$A \wedge  \neg A, 0\varoplus $} \\ $A, 0\varoplus $ \\ $\neg A, 0\varoplus $ \\ $ \varotimes  $}  ]


\begin{quote} 
(5) $ \neg (A \vee  \neg A)\nvdash  A \wedge  \neg A $
\end{quote} 
\bigskip

\Tree[.{\framebox{$\neg (A \vee  \neg A), 0\varoplus $} \\ \framebox{$A \wedge  \neg A, 0\varominus $} \\ $0\mathcal{R} 0$ \\ \framebox{$\neg (A \wedge  \neg A), 0\varoplus $} \\ $A, 0\varominus $ \\ $\neg A, 0\varominus $} [.{$A, 0\varominus $}  ] 
[.{$\neg A, 0\varominus $}  ]  ]

\bigskip

Counter Model: 

\bigskip
\noindent $\mathcal{W} = \{ w_0\} $\\
$\mathcal{R} = \{ \langle w_0,w_0 \rangle \} $\\
$ \mathcal{\nu}_{w_0}(A)=.5 $ \\
\bigskip




\begin{quote} 
(6) $ B\nvdash  (A \wedge  A) \vee  (\neg A \wedge  \neg A) $
\end{quote} 
\bigskip

\Tree[.{$B, 0\varoplus $ \\ \framebox{$(A \wedge  A) \vee  (\neg A \wedge  \neg A), 0\varominus $} \\ $0\mathcal{R} 0$ \\ \framebox{$\neg ((A \wedge  A) \vee  (\neg A \wedge  \neg A)), 0\varoplus $} \\ \framebox{$A \wedge  A, 0\varominus $} \\ \framebox{$\neg A \wedge  \neg A, 0\varominus $} \\ \framebox{$\neg (A \wedge  A), 0\varoplus $} \\ \framebox{$\neg (\neg A \wedge  \neg A), 0\varoplus $}} [.{$A, 0\varominus $} [.{$\neg A, 0\varominus $}  ] 
[.{$\neg A, 0\varominus $}  ]  ] 
[.{$A, 0\varominus $} [.{$\neg A, 0\varominus $}  ] 
[.{$\neg A, 0\varominus $}  ]  ]  ]

\bigskip

Counter Model: 

\bigskip
\noindent $\mathcal{W} = \{ w_0\} $\\
$\mathcal{R} = \{ \langle w_0,w_0 \rangle \} $\\
$ \mathcal{\nu}_{w_0}(B)=1 $ \\
$ \mathcal{\nu}_{w_0}(A)=.5 $ \\
\bigskip




\begin{quote} 
(7) $ B\nvdash  (A \vee  A) \vee  (\neg A \vee  \neg A) $
\end{quote} 
\bigskip

\Tree[.{$B, 0\varoplus $ \\ \framebox{$(A \vee  A) \vee  (\neg A \vee  \neg A), 0\varominus $} \\ $0\mathcal{R} 0$ \\ \framebox{$\neg ((A \vee  A) \vee  (\neg A \vee  \neg A)), 0\varoplus $} \\ \framebox{$A \vee  A, 0\varominus $} \\ \framebox{$\neg A \vee  \neg A, 0\varominus $} \\ \framebox{$\neg (A \vee  A), 0\varoplus $} \\ \framebox{$\neg (\neg A \vee  \neg A), 0\varoplus $} \\ $A, 0\varominus $ \\ $\neg A, 0\varominus $}  ]

\bigskip

Counter Model: 

\bigskip
\noindent $\mathcal{W} = \{ w_0\} $\\
$\mathcal{R} = \{ \langle w_0,w_0 \rangle \} $\\
$ \mathcal{\nu}_{w_0}(B)=1 $ \\
$ \mathcal{\nu}_{w_0}(A)=.5 $ \\
\bigskip




\begin{quote} 
(8a) $ A \wedge  B\vdash  B \wedge  A $
\end{quote} 
\bigskip

\Tree[.{\framebox{$A \wedge  B, 0\varoplus $} \\ \framebox{$B \wedge  A, 0\varominus $} \\ $0\mathcal{R} 0$ \\ $A, 0\varoplus $ \\ $B, 0\varoplus $ \\ \framebox{$\neg (B \wedge  A), 0\varoplus $}} [.{$B, 0\varominus $ \\ $ \varotimes  $}  ] 
[.{$A, 0\varominus $ \\ $ \varotimes  $}  ]  ]


\begin{quote} 
(8b) $ B \wedge  A\vdash  A \wedge  B $
\end{quote} 
\bigskip

\Tree[.{\framebox{$B \wedge  A, 0\varoplus $} \\ \framebox{$A \wedge  B, 0\varominus $} \\ $0\mathcal{R} 0$ \\ $B, 0\varoplus $ \\ $A, 0\varoplus $ \\ \framebox{$\neg (A \wedge  B), 0\varoplus $}} [.{$A, 0\varominus $ \\ $ \varotimes  $}  ] 
[.{$B, 0\varominus $ \\ $ \varotimes  $}  ]  ]


\begin{quote} 
(9a) $ A \vee  B\vdash  B \vee  A $
\end{quote} 
\bigskip

\Tree[.{\framebox{$A \vee  B, 0\varoplus $} \\ \framebox{$B \vee  A, 0\varominus $} \\ $0\mathcal{R} 0$ \\ \framebox{$\neg (B \vee  A), 0\varoplus $} \\ $B, 0\varominus $ \\ $A, 0\varominus $} [.{$A, 0\varoplus $ \\ $ \varotimes  $}  ] 
[.{$B, 0\varoplus $ \\ $ \varotimes  $}  ]  ]


\begin{quote} 
(9b) $ B \vee  A\vdash  A \vee  B $
\end{quote} 
\bigskip

\Tree[.{\framebox{$B \vee  A, 0\varoplus $} \\ \framebox{$A \vee  B, 0\varominus $} \\ $0\mathcal{R} 0$ \\ \framebox{$\neg (A \vee  B), 0\varoplus $} \\ $A, 0\varominus $ \\ $B, 0\varominus $} [.{$B, 0\varoplus $ \\ $ \varotimes  $}  ] 
[.{$A, 0\varoplus $ \\ $ \varotimes  $}  ]  ]


\begin{quote} 
(10a) $ A \wedge  (B \wedge  C)\vdash  (A \wedge  B) \wedge  C $
\end{quote} 
\bigskip

\Tree[.{\framebox{$A \wedge  (B \wedge  C), 0\varoplus $} \\ \framebox{$(A \wedge  B) \wedge  C, 0\varominus $} \\ $0\mathcal{R} 0$ \\ $A, 0\varoplus $ \\ \framebox{$B \wedge  C, 0\varoplus $} \\ $B, 0\varoplus $ \\ $C, 0\varoplus $ \\ \framebox{$\neg ((A \wedge  B) \wedge  C), 0\varoplus $}} [.{$C, 0\varominus $ \\ $ \varotimes  $}  ] 
[.{\framebox{$A \wedge  B, 0\varominus $} \\ \framebox{$\neg (A \wedge  B), 0\varoplus $}} [.{$A, 0\varominus $ \\ $ \varotimes  $}  ] 
[.{$B, 0\varominus $ \\ $ \varotimes  $}  ]  ]  ]


\begin{quote} 
(10b) $ (A \wedge  B) \wedge  C\vdash  A \wedge  (B \wedge  C) $
\end{quote} 
\bigskip

\Tree[.{\framebox{$(A \wedge  B) \wedge  C, 0\varoplus $} \\ \framebox{$A \wedge  (B \wedge  C), 0\varominus $} \\ $0\mathcal{R} 0$ \\ \framebox{$A \wedge  B, 0\varoplus $} \\ $C, 0\varoplus $ \\ $A, 0\varoplus $ \\ $B, 0\varoplus $ \\ \framebox{$\neg (A \wedge  (B \wedge  C)), 0\varoplus $}} [.{$A, 0\varominus $ \\ $ \varotimes  $}  ] 
[.{\framebox{$B \wedge  C, 0\varominus $} \\ \framebox{$\neg (B \wedge  C), 0\varoplus $}} [.{$B, 0\varominus $ \\ $ \varotimes  $}  ] 
[.{$C, 0\varominus $ \\ $ \varotimes  $}  ]  ]  ]


\begin{quote} 
(11a) $ A \vee  (B \vee  C)\vdash  (A \vee  B) \vee  C $
\end{quote} 
\bigskip

\Tree[.{\framebox{$A \vee  (B \vee  C), 0\varoplus $} \\ \framebox{$(A \vee  B) \vee  C, 0\varominus $} \\ $0\mathcal{R} 0$ \\ \framebox{$\neg ((A \vee  B) \vee  C), 0\varoplus $} \\ \framebox{$A \vee  B, 0\varominus $} \\ $C, 0\varominus $ \\ \framebox{$\neg (A \vee  B), 0\varoplus $} \\ $A, 0\varominus $ \\ $B, 0\varominus $} [.{$A, 0\varoplus $ \\ $ \varotimes  $}  ] 
[.{\framebox{$B \vee  C, 0\varoplus $}} [.{$B, 0\varoplus $ \\ $ \varotimes  $}  ] 
[.{$C, 0\varoplus $ \\ $ \varotimes  $}  ]  ]  ]


\begin{quote} 
(11b) $ (A \vee  B) \vee  C\vdash  A \vee  (B \vee  C) $
\end{quote} 
\bigskip

\Tree[.{\framebox{$(A \vee  B) \vee  C, 0\varoplus $} \\ \framebox{$A \vee  (B \vee  C), 0\varominus $} \\ $0\mathcal{R} 0$ \\ \framebox{$\neg (A \vee  (B \vee  C)), 0\varoplus $} \\ $A, 0\varominus $ \\ \framebox{$B \vee  C, 0\varominus $} \\ \framebox{$\neg (B \vee  C), 0\varoplus $} \\ $B, 0\varominus $ \\ $C, 0\varominus $} [.{$C, 0\varoplus $ \\ $ \varotimes  $}  ] 
[.{\framebox{$A \vee  B, 0\varoplus $}} [.{$A, 0\varoplus $ \\ $ \varotimes  $}  ] 
[.{$B, 0\varoplus $ \\ $ \varotimes  $}  ]  ]  ]


\begin{quote} 
(12a) $ A\vdash  A \wedge  A $
\end{quote} 
\bigskip

\Tree[.{$A, 0\varoplus $ \\ \framebox{$A \wedge  A, 0\varominus $} \\ $0\mathcal{R} 0$ \\ \framebox{$\neg (A \wedge  A), 0\varoplus $}} [.{$A, 0\varominus $ \\ $ \varotimes  $}  ] 
[.{$A, 0\varominus $ \\ $ \varotimes  $}  ]  ]


\begin{quote} 
(12b) $ A \wedge  A\vdash  A $
\end{quote} 
\bigskip

\Tree[.{\framebox{$A \wedge  A, 0\varoplus $} \\ $A, 0\varominus $ \\ $0\mathcal{R} 0$ \\ $A, 0\varoplus $ \\ $ \varotimes  $}  ]


\begin{quote} 
(13a) $ A\vdash  A \vee  A $
\end{quote} 
\bigskip

\Tree[.{$A, 0\varoplus $ \\ \framebox{$A \vee  A, 0\varominus $} \\ $0\mathcal{R} 0$ \\ \framebox{$\neg (A \vee  A), 0\varoplus $} \\ $A, 0\varominus $ \\ $ \varotimes  $}  ]


\begin{quote} 
(13b) $ A \vee  A\vdash  A $
\end{quote} 
\bigskip

\Tree[.{\framebox{$A \vee  A, 0\varoplus $} \\ $A, 0\varominus $ \\ $0\mathcal{R} 0$} [.{$A, 0\varoplus $ \\ $ \varotimes  $}  ] 
[.{$A, 0\varoplus $ \\ $ \varotimes  $}  ]  ]


\begin{quote} 
(14a) $ A \wedge  (B \vee  C)\vdash  (A \wedge  B) \vee  (A \wedge  C) $
\end{quote} 
\bigskip

\Tree[.{\framebox{$A \wedge  (B \vee  C), 0\varoplus $} \\ \framebox{$(A \wedge  B) \vee  (A \wedge  C), 0\varominus $} \\ $0\mathcal{R} 0$ \\ $A, 0\varoplus $ \\ \framebox{$B \vee  C, 0\varoplus $} \\ \framebox{$\neg ((A \wedge  B) \vee  (A \wedge  C)), 0\varoplus $} \\ \framebox{$A \wedge  B, 0\varominus $} \\ \framebox{$A \wedge  C, 0\varominus $} \\ \framebox{$\neg (A \wedge  B), 0\varoplus $} \\ \framebox{$\neg (A \wedge  C), 0\varoplus $}} [.{$B, 0\varoplus $} [.{$A, 0\varominus $ \\ $ \varotimes  $}  ] 
[.{$B, 0\varominus $ \\ $ \varotimes  $}  ]  ] 
[.{$C, 0\varoplus $} [.{$A, 0\varominus $ \\ $ \varotimes  $}  ] 
[.{$B, 0\varominus $} [.{$A, 0\varominus $ \\ $ \varotimes  $}  ] 
[.{$C, 0\varominus $ \\ $ \varotimes  $}  ]  ]  ]  ]


\begin{quote} 
(14b) $ (A \wedge  B) \vee  (A \wedge  C)\vdash  A \wedge  (B \vee  C) $
\end{quote} 
\bigskip

\Tree[.{\framebox{$(A \wedge  B) \vee  (A \wedge  C), 0\varoplus $} \\ \framebox{$A \wedge  (B \vee  C), 0\varominus $} \\ $0\mathcal{R} 0$ \\ \framebox{$\neg (A \wedge  (B \vee  C)), 0\varoplus $}} [.{\framebox{$A \wedge  B, 0\varoplus $} \\ $A, 0\varoplus $ \\ $B, 0\varoplus $} [.{$A, 0\varominus $ \\ $ \varotimes  $}  ] 
[.{\framebox{$B \vee  C, 0\varominus $} \\ \framebox{$\neg (B \vee  C), 0\varoplus $} \\ $B, 0\varominus $ \\ $C, 0\varominus $ \\ $ \varotimes  $}  ]  ] 
[.{\framebox{$A \wedge  C, 0\varoplus $} \\ $A, 0\varoplus $ \\ $C, 0\varoplus $} [.{$A, 0\varominus $ \\ $ \varotimes  $}  ] 
[.{\framebox{$B \vee  C, 0\varominus $} \\ \framebox{$\neg (B \vee  C), 0\varoplus $} \\ $B, 0\varominus $ \\ $C, 0\varominus $ \\ $ \varotimes  $}  ]  ]  ]


\begin{quote} 
(15a) $ A \vee  (B \wedge  C)\vdash  (A \vee  B) \wedge  (A \vee  C) $
\end{quote} 
\bigskip

\Tree[.{\framebox{$A \vee  (B \wedge  C), 0\varoplus $} \\ \framebox{$(A \vee  B) \wedge  (A \vee  C), 0\varominus $} \\ $0\mathcal{R} 0$ \\ \framebox{$\neg ((A \vee  B) \wedge  (A \vee  C)), 0\varoplus $}} [.{$A, 0\varoplus $} [.{\framebox{$A \vee  B, 0\varominus $} \\ \framebox{$\neg (A \vee  B), 0\varoplus $} \\ $A, 0\varominus $ \\ $B, 0\varominus $ \\ $ \varotimes  $}  ] 
[.{\framebox{$A \vee  C, 0\varominus $} \\ \framebox{$\neg (A \vee  C), 0\varoplus $} \\ $A, 0\varominus $ \\ $C, 0\varominus $ \\ $ \varotimes  $}  ]  ] 
[.{\framebox{$B \wedge  C, 0\varoplus $} \\ $B, 0\varoplus $ \\ $C, 0\varoplus $} [.{\framebox{$A \vee  B, 0\varominus $} \\ \framebox{$\neg (A \vee  B), 0\varoplus $} \\ $A, 0\varominus $ \\ $B, 0\varominus $ \\ $ \varotimes  $}  ] 
[.{\framebox{$A \vee  C, 0\varominus $} \\ \framebox{$\neg (A \vee  C), 0\varoplus $} \\ $A, 0\varominus $ \\ $C, 0\varominus $ \\ $ \varotimes  $}  ]  ]  ]


\begin{quote} 
(15b) $ (A \vee  B) \wedge  (A \vee  C)\vdash  A \vee  (B \wedge  C) $
\end{quote} 
\bigskip

\Tree[.{\framebox{$(A \vee  B) \wedge  (A \vee  C), 0\varoplus $} \\ \framebox{$A \vee  (B \wedge  C), 0\varominus $} \\ $0\mathcal{R} 0$ \\ \framebox{$A \vee  B, 0\varoplus $} \\ \framebox{$A \vee  C, 0\varoplus $} \\ \framebox{$\neg (A \vee  (B \wedge  C)), 0\varoplus $} \\ $A, 0\varominus $ \\ \framebox{$B \wedge  C, 0\varominus $} \\ \framebox{$\neg (B \wedge  C), 0\varoplus $}} [.{$A, 0\varoplus $ \\ $ \varotimes  $}  ] 
[.{$B, 0\varoplus $} [.{$A, 0\varoplus $ \\ $ \varotimes  $}  ] 
[.{$C, 0\varoplus $} [.{$B, 0\varominus $ \\ $ \varotimes  $}  ] 
[.{$C, 0\varominus $ \\ $ \varotimes  $}  ]  ]  ]  ]


\begin{quote} 
(16) $ \{A \vee  B, \neg A \} \vdash  B $
\end{quote} 
\bigskip

\Tree[.{\framebox{$A \vee  B, 0\varoplus $} \\ $\neg A, 0\varoplus $ \\ $B, 0\varominus $ \\ $0\mathcal{R} 0$} [.{$A, 0\varoplus $ \\ $ \varotimes  $}  ] 
[.{$B, 0\varoplus $ \\ $ \varotimes  $}  ]  ]