\documentclass{article}
\usepackage{latexsym, qtree, stmaryrd}
\usepackage{amssymb}
\begin{document}


\bigskip
\begin{quote} 
(1) $ A \vee  B\vdash  \neg (\neg (A \wedge  A) \wedge  \neg (B \wedge  B)) $
\end{quote} 
\bigskip

\Tree[.{\framebox{$A \vee  B, 0\varoplus $} \\ \framebox{$\neg (\neg (A \wedge  A) \wedge  \neg (B \wedge  B)), 0\varominus $} \\ $0\mathcal{R} 0$ \\ \framebox{$\neg (A \wedge  A) \wedge  \neg (B \wedge  B), 0\varoplus $} \\ \framebox{$\neg (A \wedge  A), 0\varoplus $} \\ \framebox{$\neg (B \wedge  B), 0\varoplus $}} [.{$A, 0\varoplus $} [.{$A, 0\varominus $ \\ $ \varotimes  $}  ] 
[.{$A, 0\varominus $ \\ $ \varotimes  $}  ]  ] 
[.{$B, 0\varoplus $} [.{$A, 0\varominus $} [.{$B, 0\varominus $ \\ $ \varotimes  $}  ] 
[.{$B, 0\varominus $ \\ $ \varotimes  $}  ]  ] 
[.{$A, 0\varominus $} [.{$B, 0\varominus $ \\ $ \varotimes  $}  ] 
[.{$B, 0\varominus $ \\ $ \varotimes  $}  ]  ]  ]  ]

\bigskip
\begin{quote} 
(2) $ \neg (\neg (A \wedge  A) \wedge  \neg (B \wedge  B))\vdash  A \vee  B $
\end{quote} 
\bigskip

\Tree[.{\framebox{$\neg (\neg (A \wedge  A) \wedge  \neg (B \wedge  B)), 0\varoplus $} \\ \framebox{$A \vee  B, 0\varominus $} \\ $0\mathcal{R} 0$ \\ \framebox{$\neg (A \vee  B), 0\varoplus $} \\ $A, 0\varominus $ \\ $B, 0\varominus $} [.{\framebox{$\neg (A \wedge  A), 0\varominus $} \\ \framebox{$A \wedge  A, 0\varoplus $} \\ $A, 0\varoplus $ \\ $ \varotimes  $}  ] 
[.{\framebox{$\neg (B \wedge  B), 0\varominus $} \\ \framebox{$B \wedge  B, 0\varoplus $} \\ $B, 0\varoplus $ \\ $ \varotimes  $}  ]  ]


 \end{document}