%%%%%%%%%%%%%%%%%% ARGUMENT LIST %%%%%%%%%%%%%%%%%%%%

\noindent \textbf{Material Conditional}

\begin{enumerate}
\setcounter{enumi}{\value{enumi_saved}}
\item $ B\nvdash  A \supset  A $\hfill\emph{ (Identity)}  
\item $ B\vdash  (A \wedge  A) \supset  A $\hfill\emph{ (Identity - Restricted)}  
\item $ \{A, A \supset  B \} \vdash  B $\hfill\emph{ (Modus Ponens)}  
\item $ C\vdash  (A \wedge  (A \supset  B)) \supset  B $\hfill\emph{ (Pseudo Modus Ponens)}  
\item $ \{\neg B, A \supset  B \} \vdash  \neg A $\hfill\emph{ (Modus Tollens)}  
\item $ C\vdash  (\neg B \wedge  (A \supset  B)) \supset  \neg A $\hfill\emph{ (Pseudo Modus Tollens)}  
\item $ \{A \supset  B, B \supset  C \} \vdash  A \supset  C $\hfill\emph{ (Hypothetical Syllogism)}  
\item $ A \supset  (A \supset  B)\leftvdash\rightvdash  A \supset  B $ \hfill\emph{ (Contraction)}  
\item $ C\vdash  (A \supset  (A \supset  B)) \supset  (A \supset  B) $\hfill\emph{ (Pseudo Contraction)}  
\item $ A \supset  B\leftvdash\rightvdash  \neg B \supset  \neg A $ \hfill\emph{ (Contraposition)}  
\item $ C\vdash  (A \supset  B) \supset  (\neg B \supset  \neg A) $\hfill\emph{ (Pseudo Contraposition)}  
\item $ A \supset  (B \supset  C)\leftvdash\rightvdash  (A \wedge  B) \supset  C $ \hfill\emph{ (Exportation)}  
\item $ \neg A\vdash  A \supset  B $\hfill\emph{ }  
\item $ \neg (A \supset  B)\nvdash  \neg B $\hfill\emph{ }  
\item $ A\vdash  B \supset  A $\hfill\emph{ }  
\item $ A \supset  B\vdash  (A \wedge  C) \supset  B $\hfill\emph{ }  
\item $ (A \wedge  B) \supset  C\nvdash  (A \supset  C) \vee  (B \supset  C) $\hfill\emph{ }  
\setcounter{enumi_saved}{\value{enumi}}
\end{enumerate}


%%%%%%%%%%%%%%%%%%%%% TABLEAUX %%%%%%%%%%%%%%%%%%%%%




\begin{quote} 
(23) $ B\nvdash  A \supset  A $
\end{quote} 
\bigskip

\Tree[.{$B, 0\varoplus $ \\ \framebox{$A \supset  A, 0\varominus $} \\ $0\mathcal{R} 0$ \\ \framebox{$\neg (A \supset  A), 0\varoplus $} \\ $\neg A, 0\varominus $ \\ $A, 0\varominus $}  ]

\bigskip

Counter Model: 

\bigskip
\noindent $\mathcal{W} = \{ w_0\} $\\
$\mathcal{R} = \{ \langle w_0,w_0 \rangle \} $\\
$ \mathcal{\nu}_{w_0}(B)=1 $ \\
$ \mathcal{\nu}_{w_0}(A)=.5 $ \\
\bigskip




\begin{quote} 
(24) $ B\vdash  (A \wedge  A) \supset  A $
\end{quote} 
\bigskip

\Tree[.{$B, 0\varoplus $ \\ \framebox{$(A \wedge  A) \supset  A, 0\varominus $} \\ $0\mathcal{R} 0$ \\ \framebox{$\neg ((A \wedge  A) \supset  A), 0\varoplus $} \\ \framebox{$\neg (A \wedge  A), 0\varominus $} \\ $A, 0\varominus $ \\ \framebox{$A \wedge  A, 0\varoplus $} \\ $A, 0\varoplus $ \\ $ \varotimes  $}  ]


\begin{quote} 
(25) $ \{A, A \supset  B \} \vdash  B $
\end{quote} 
\bigskip

\Tree[.{$A, 0\varoplus $ \\ \framebox{$A \supset  B, 0\varoplus $} \\ $B, 0\varominus $ \\ $0\mathcal{R} 0$} [.{$\neg A, 0\varoplus $ \\ $ \varotimes  $}  ] 
[.{$B, 0\varoplus $ \\ $ \varotimes  $}  ]  ]


\begin{quote} 
(26) $ C\vdash  (A \wedge  (A \supset  B)) \supset  B $
\end{quote} 
\bigskip

\Tree[.{$C, 0\varoplus $ \\ \framebox{$(A \wedge  (A \supset  B)) \supset  B, 0\varominus $} \\ $0\mathcal{R} 0$ \\ \framebox{$\neg ((A \wedge  (A \supset  B)) \supset  B), 0\varoplus $} \\ \framebox{$\neg (A \wedge  (A \supset  B)), 0\varominus $} \\ $B, 0\varominus $ \\ \framebox{$A \wedge  (A \supset  B), 0\varoplus $} \\ $A, 0\varoplus $ \\ \framebox{$A \supset  B, 0\varoplus $}} [.{$\neg A, 0\varoplus $ \\ $ \varotimes  $}  ] 
[.{$B, 0\varoplus $ \\ $ \varotimes  $}  ]  ]


\begin{quote} 
(27) $ \{\neg B, A \supset  B \} \vdash  \neg A $
\end{quote} 
\bigskip

\Tree[.{$\neg B, 0\varoplus $ \\ \framebox{$A \supset  B, 0\varoplus $} \\ $\neg A, 0\varominus $ \\ $0\mathcal{R} 0$} [.{$\neg A, 0\varoplus $ \\ $ \varotimes  $}  ] 
[.{$B, 0\varoplus $ \\ $ \varotimes  $}  ]  ]


\begin{quote} 
(28) $ C\vdash  (\neg B \wedge  (A \supset  B)) \supset  \neg A $
\end{quote} 
\bigskip

\Tree[.{$C, 0\varoplus $ \\ \framebox{$(\neg B \wedge  (A \supset  B)) \supset  \neg A, 0\varominus $} \\ $0\mathcal{R} 0$ \\ \framebox{$\neg ((\neg B \wedge  (A \supset  B)) \supset  \neg A), 0\varoplus $} \\ \framebox{$\neg (\neg B \wedge  (A \supset  B)), 0\varominus $} \\ $\neg A, 0\varominus $ \\ \framebox{$\neg B \wedge  (A \supset  B), 0\varoplus $} \\ $\neg B, 0\varoplus $ \\ \framebox{$A \supset  B, 0\varoplus $}} [.{$\neg A, 0\varoplus $ \\ $ \varotimes  $}  ] 
[.{$B, 0\varoplus $ \\ $ \varotimes  $}  ]  ]


\begin{quote} 
(29) $ \{A \supset  B, B \supset  C \} \vdash  A \supset  C $
\end{quote} 
\bigskip

\Tree[.{\framebox{$A \supset  B, 0\varoplus $} \\ \framebox{$B \supset  C, 0\varoplus $} \\ \framebox{$A \supset  C, 0\varominus $} \\ $0\mathcal{R} 0$ \\ \framebox{$\neg (A \supset  C), 0\varoplus $} \\ $\neg A, 0\varominus $ \\ $C, 0\varominus $} [.{$\neg A, 0\varoplus $ \\ $ \varotimes  $}  ] 
[.{$B, 0\varoplus $} [.{$\neg B, 0\varoplus $ \\ $ \varotimes  $}  ] 
[.{$C, 0\varoplus $ \\ $ \varotimes  $}  ]  ]  ]


\begin{quote} 
(30a) $ A \supset  (A \supset  B)\vdash  A \supset  B $
\end{quote} 
\bigskip

\Tree[.{\framebox{$A \supset  (A \supset  B), 0\varoplus $} \\ \framebox{$A \supset  B, 0\varominus $} \\ $0\mathcal{R} 0$ \\ \framebox{$\neg (A \supset  B), 0\varoplus $} \\ $\neg A, 0\varominus $ \\ $B, 0\varominus $} [.{$\neg A, 0\varoplus $ \\ $ \varotimes  $}  ] 
[.{$A \supset  B, 0\varoplus $ \\ $ \varotimes  $}  ]  ]


\begin{quote} 
(30b) $ A \supset  B\vdash  A \supset  (A \supset  B) $
\end{quote} 
\bigskip

\Tree[.{$A \supset  B, 0\varoplus $ \\ \framebox{$A \supset  (A \supset  B), 0\varominus $} \\ $0\mathcal{R} 0$ \\ \framebox{$\neg (A \supset  (A \supset  B)), 0\varoplus $} \\ $\neg A, 0\varominus $ \\ $A \supset  B, 0\varominus $ \\ $ \varotimes  $}  ]


\begin{quote} 
(31) $ C\vdash  (A \supset  (A \supset  B)) \supset  (A \supset  B) $
\end{quote} 
\bigskip

\Tree[.{$C, 0\varoplus $ \\ \framebox{$(A \supset  (A \supset  B)) \supset  (A \supset  B), 0\varominus $} \\ $0\mathcal{R} 0$ \\ \framebox{$\neg ((A \supset  (A \supset  B)) \supset  (A \supset  B)), 0\varoplus $} \\ \framebox{$\neg (A \supset  (A \supset  B)), 0\varominus $} \\ \framebox{$A \supset  B, 0\varominus $} \\ \framebox{$\neg (A \supset  B), 0\varoplus $} \\ $\neg A, 0\varominus $ \\ $B, 0\varominus $ \\ \framebox{$A \supset  (A \supset  B), 0\varoplus $}} [.{$\neg A, 0\varoplus $ \\ $ \varotimes  $}  ] 
[.{$A \supset  B, 0\varoplus $ \\ $ \varotimes  $}  ]  ]


\begin{quote} 
(32a) $ A \supset  B\vdash  \neg B \supset  \neg A $
\end{quote} 
\bigskip

\Tree[.{\framebox{$A \supset  B, 0\varoplus $} \\ \framebox{$\neg B \supset  \neg A, 0\varominus $} \\ $0\mathcal{R} 0$ \\ \framebox{$\neg (\neg B \supset  \neg A), 0\varoplus $} \\ \framebox{$\neg \neg B, 0\varominus $} \\ $\neg A, 0\varominus $ \\ $B, 0\varominus $} [.{$\neg A, 0\varoplus $ \\ $ \varotimes  $}  ] 
[.{$B, 0\varoplus $ \\ $ \varotimes  $}  ]  ]


\begin{quote} 
(32b) $ \neg B \supset  \neg A\vdash  A \supset  B $
\end{quote} 
\bigskip

\Tree[.{\framebox{$\neg B \supset  \neg A, 0\varoplus $} \\ \framebox{$A \supset  B, 0\varominus $} \\ $0\mathcal{R} 0$ \\ \framebox{$\neg (A \supset  B), 0\varoplus $} \\ $\neg A, 0\varominus $ \\ $B, 0\varominus $} [.{$\neg A, 0\varoplus $ \\ $ \varotimes  $}  ] 
[.{\framebox{$\neg \neg B, 0\varoplus $} \\ $B, 0\varoplus $ \\ $ \varotimes  $}  ]  ]


\begin{quote} 
(33) $ C\vdash  (A \supset  B) \supset  (\neg B \supset  \neg A) $
\end{quote} 
\bigskip

\Tree[.{$C, 0\varoplus $ \\ \framebox{$(A \supset  B) \supset  (\neg B \supset  \neg A), 0\varominus $} \\ $0\mathcal{R} 0$ \\ \framebox{$\neg ((A \supset  B) \supset  (\neg B \supset  \neg A)), 0\varoplus $} \\ \framebox{$\neg (A \supset  B), 0\varominus $} \\ \framebox{$\neg B \supset  \neg A, 0\varominus $} \\ \framebox{$\neg (\neg B \supset  \neg A), 0\varoplus $} \\ \framebox{$\neg \neg B, 0\varominus $} \\ $\neg A, 0\varominus $ \\ $B, 0\varominus $ \\ \framebox{$A \supset  B, 0\varoplus $}} [.{$\neg A, 0\varoplus $ \\ $ \varotimes  $}  ] 
[.{$B, 0\varoplus $ \\ $ \varotimes  $}  ]  ]


\begin{quote} 
(34a) $ A \supset  (B \supset  C)\vdash  (A \wedge  B) \supset  C $
\end{quote} 
\bigskip

\Tree[.{\framebox{$A \supset  (B \supset  C), 0\varoplus $} \\ \framebox{$(A \wedge  B) \supset  C, 0\varominus $} \\ $0\mathcal{R} 0$ \\ \framebox{$\neg ((A \wedge  B) \supset  C), 0\varoplus $} \\ \framebox{$\neg (A \wedge  B), 0\varominus $} \\ $C, 0\varominus $ \\ \framebox{$A \wedge  B, 0\varoplus $} \\ $A, 0\varoplus $ \\ $B, 0\varoplus $} [.{$\neg A, 0\varoplus $ \\ $ \varotimes  $}  ] 
[.{\framebox{$B \supset  C, 0\varoplus $}} [.{$\neg B, 0\varoplus $ \\ $ \varotimes  $}  ] 
[.{$C, 0\varoplus $ \\ $ \varotimes  $}  ]  ]  ]


\begin{quote} 
(34b) $ (A \wedge  B) \supset  C\nvdash  A \supset  (B \supset  C) $
\end{quote} 
\bigskip

\Tree[.{\framebox{$(A \wedge  B) \supset  C, 0\varoplus $} \\ \framebox{$A \supset  (B \supset  C), 0\varominus $} \\ $0\mathcal{R} 0$ \\ \framebox{$\neg (A \supset  (B \supset  C)), 0\varoplus $} \\ $\neg A, 0\varominus $ \\ \framebox{$B \supset  C, 0\varominus $} \\ \framebox{$\neg (B \supset  C), 0\varoplus $} \\ $\neg B, 0\varominus $ \\ $C, 0\varominus $} [.{$C, 0\varoplus $ \\ $ \varotimes  $}  ] 
[.{\framebox{$\neg (A \wedge  B), 0\varoplus $}} [.{$A, 0\varominus $}  ] 
[.{$B, 0\varominus $}  ]  ]  ]

\bigskip

Counter Model: 

\bigskip
\noindent $\mathcal{W} = \{ w_0\} $\\
$\mathcal{R} = \{ \langle w_0,w_0 \rangle \} $\\
$ \mathcal{\nu}_{w_0}(C)=0 $ \\
$ \mathcal{\nu}_{w_0}(A)=.5 $ \\
\bigskip




\begin{quote} 
(35) $ \neg A\vdash  A \supset  B $
\end{quote} 
\bigskip

\Tree[.{$\neg A, 0\varoplus $ \\ \framebox{$A \supset  B, 0\varominus $} \\ $0\mathcal{R} 0$ \\ \framebox{$\neg (A \supset  B), 0\varoplus $} \\ $\neg A, 0\varominus $ \\ $B, 0\varominus $ \\ $ \varotimes  $}  ]


\begin{quote} 
(36) $ \neg (A \supset  B)\nvdash  \neg B $
\end{quote} 
\bigskip

\Tree[.{\framebox{$\neg (A \supset  B), 0\varoplus $} \\ $\neg B, 0\varominus $ \\ $0\mathcal{R} 0$ \\ $\neg A, 0\varominus $ \\ $B, 0\varominus $}  ]

\bigskip

Counter Model: 

\bigskip
\noindent $\mathcal{W} = \{ w_0\} $\\
$\mathcal{R} = \{ \langle w_0,w_0 \rangle \} $\\
$ \mathcal{\nu}_{w_0}(B)=.5 $ \\
\bigskip




\begin{quote} 
(37) $ A\vdash  B \supset  A $
\end{quote} 
\bigskip

\Tree[.{$A, 0\varoplus $ \\ \framebox{$B \supset  A, 0\varominus $} \\ $0\mathcal{R} 0$ \\ \framebox{$\neg (B \supset  A), 0\varoplus $} \\ $\neg B, 0\varominus $ \\ $A, 0\varominus $ \\ $ \varotimes  $}  ]


\begin{quote} 
(38) $ A \supset  B\vdash  (A \wedge  C) \supset  B $
\end{quote} 
\bigskip

\Tree[.{\framebox{$A \supset  B, 0\varoplus $} \\ \framebox{$(A \wedge  C) \supset  B, 0\varominus $} \\ $0\mathcal{R} 0$ \\ \framebox{$\neg ((A \wedge  C) \supset  B), 0\varoplus $} \\ \framebox{$\neg (A \wedge  C), 0\varominus $} \\ $B, 0\varominus $ \\ \framebox{$A \wedge  C, 0\varoplus $} \\ $A, 0\varoplus $ \\ $C, 0\varoplus $} [.{$\neg A, 0\varoplus $ \\ $ \varotimes  $}  ] 
[.{$B, 0\varoplus $ \\ $ \varotimes  $}  ]  ]


\begin{quote} 
(39) $ (A \wedge  B) \supset  C\nvdash  (A \supset  C) \vee  (B \supset  C) $
\end{quote} 
\bigskip

\Tree[.{\framebox{$(A \wedge  B) \supset  C, 0\varoplus $} \\ \framebox{$(A \supset  C) \vee  (B \supset  C), 0\varominus $} \\ $0\mathcal{R} 0$ \\ \framebox{$\neg ((A \supset  C) \vee  (B \supset  C)), 0\varoplus $} \\ \framebox{$A \supset  C, 0\varominus $} \\ \framebox{$B \supset  C, 0\varominus $} \\ \framebox{$\neg (A \supset  C), 0\varoplus $} \\ \framebox{$\neg (B \supset  C), 0\varoplus $} \\ $\neg A, 0\varominus $ \\ $C, 0\varominus $ \\ $\neg B, 0\varominus $} [.{$C, 0\varominus $} [.{$C, 0\varoplus $ \\ $ \varotimes  $}  ] 
[.{\framebox{$\neg (A \wedge  B), 0\varoplus $}} [.{$A, 0\varominus $}  ] 
[.{$B, 0\varominus $}  ]  ]  ]  ]

\bigskip

Counter Model: 

\bigskip
\noindent $\mathcal{W} = \{ w_0\} $\\
$\mathcal{R} = \{ \langle w_0,w_0 \rangle \} $\\
$ \mathcal{\nu}_{w_0}(C)=0 $ \\
$ \mathcal{\nu}_{w_0}(A)=.5 $ \\
\bigskip

